Prove inverse round trip for bytestring packing and add serialisation of basic building blocks

isabelle/Semantics.thy
@@ -21,7 +21,6 @@ datatype Party = PubKey ByteString
 
 type_synonym AccountId = Party
 
-
 (* BEGIN Proof of linorder for Party *)
 fun less_eq_Party :: "Party \<Rightarrow> Party \<Rightarrow> bool" where
 "less_eq_Party (PubKey _) (Role _) = True" |
@@ -106,6 +105,59 @@ qed
 end
 (* END Proof of linorder for Party *)
 
+fun partyToByteString :: "Party \<Rightarrow> ByteString" where
+"partyToByteString (PubKey x) = (positiveIntToByteString 0) @ (packByteString x)" |
+"partyToByteString (Role x) = (positiveIntToByteString 1) @ (packByteString x)"
+
+fun byteStringToParty :: "ByteString \<Rightarrow> (Party \<times> ByteString) option" where
+"byteStringToParty x =
+  (case byteStringToPositiveInt x of
+     None \<Rightarrow> None
+   | Some (y, t1) \<Rightarrow> (case getByteString t1 of
+                        None \<Rightarrow> None
+                      | Some (z, t2) \<Rightarrow> (if y = 0
+                                         then Some (PubKey z, t2)
+                                         else (if y = 1
+                                               then Some (Role z, t2)
+                                               else None))))"
+
+lemma partyToByteStringToParty : "byteStringToParty ((partyToByteString x) @ y) = Some (x, y)"
+  apply (cases x)
+  subgoal for x
+    apply (cases "byteStringToPositiveInt (positiveIntToByteString 0 @ packByteString x @ y)")
+    apply simp
+    subgoal for a
+      apply (cases a)
+      subgoal for aa ab
+      apply (simp del:byteStringToPositiveInt.simps positiveIntToByteString.simps packByteString.simps getByteString.simps)
+        using positiveIntToByteStringToPositiveInt by force
+      done
+    done
+  subgoal for x
+    apply (cases "byteStringToPositiveInt (positiveIntToByteString 1 @ packByteString x @ y)")
+    apply (simp del:byteStringToPositiveInt.simps positiveIntToByteString.simps packByteString.simps getByteString.simps)
+    apply simp
+    subgoal for a
+      apply (cases a)
+      subgoal for aa ab
+      apply (simp del:byteStringToPositiveInt.simps positiveIntToByteString.simps packByteString.simps getByteString.simps)
+        using positiveIntToByteStringToPositiveInt by force
+      done
+    done
+  done
+
+
+lemma byteStringToParty_inverseRoundtrip : "byteStringToParty x = Some (a, b) \<Longrightarrow> partyToByteString a @ b = x"
+  apply (simp del:byteStringToPositiveInt.simps getByteString.simps split:option.splits prod.splits)
+  subgoal for x2 x1 x2a x2b x1a x2c
+    apply (cases "x1 = 0")
+    apply (simp del:byteStringToPositiveInt.simps getByteString.simps split:option.splits prod.splits)
+    apply (metis addAndGetByteString_inverseRoundtrip append_eq_appendI byteStrintToPositiveInt_inverseRoundtrip partyToByteString.simps(1))
+    apply (cases "x1 = 1")
+    apply (metis addAndGetByteString_inverseRoundtrip append_eq_appendI byteStrintToPositiveInt_inverseRoundtrip old.prod.inject option.inject partyToByteString.simps(2))
+    by simp
+  done
+
 datatype Token = Token CurrencySymbol TokenName
 
 (* BEGIN Proof of linorder for Token *)
@@ -158,6 +210,29 @@ next
 qed
 end
 (* END Proof of linorder for Token *)
+
+fun tokenToByteString :: "Token \<Rightarrow> ByteString" where
+"tokenToByteString (Token tn cs) = (packByteString tn) @ (packByteString cs)"
+
+fun byteStringToToken :: "ByteString \<Rightarrow> (Token \<times> ByteString) option" where
+"byteStringToToken x =
+  (case getByteString x of
+      None \<Rightarrow> None
+    | Some (tn, t1) \<Rightarrow> (case getByteString t1 of
+                          None \<Rightarrow> None
+                        | Some (cs, t2) \<Rightarrow> Some (Token tn cs, t2)))"
+
+lemma tokenToByteStringToToken : "byteStringToToken ((tokenToByteString x) @ y) = Some (x, y)"
+  apply (cases x)
+  subgoal for tn cs
+    apply (auto simp only:tokenToByteString.simps byteStringToToken.simps split:option.splits prod.splits)
+  using addAndGetByteString by auto
+  done
+
+lemma byteStringToToken_inverseRoundtrip : "byteStringToToken x = Some (a, b) \<Longrightarrow> tokenToByteString a @ b = x"
+  apply (auto simp only:tokenToByteString.simps byteStringToToken.simps split:option.splits prod.splits)
+  using addAndGetByteString_inverseRoundtrip append_assoc by blast
+
 
 datatype ChoiceId = ChoiceId ChoiceName Party
 
@@ -215,6 +290,28 @@ next
 qed
 end
 (* END Proof of linorder for ChoiceId *)
+
+fun choiceIdToByteString :: "ChoiceId \<Rightarrow> ByteString" where
+"choiceIdToByteString (ChoiceId cn co) = (packByteString cn) @ (partyToByteString co)"
+
+fun byteStringToChoiceId :: "ByteString \<Rightarrow> (ChoiceId \<times> ByteString) option" where
+"byteStringToChoiceId x =
+  (case getByteString x of
+      None \<Rightarrow> None
+    | Some (cn, t1) \<Rightarrow> (case byteStringToParty t1 of
+                          None \<Rightarrow> None
+                        | Some (co, t2) \<Rightarrow> Some (ChoiceId cn co, t2)))"
+
+lemma choiceIdToByteStringToChoiceId : "byteStringToChoiceId ((choiceIdToByteString x) @ y) = Some (x, y)"
+  apply (cases x)
+  subgoal for cn co
+    apply (auto simp only:choiceIdToByteString.simps byteStringToChoiceId.simps split:option.splits prod.splits)
+    using addAndGetByteString partyToByteStringToParty by auto
+  done
+
+lemma byteStringToChoiceId_inverseRoundtrip : "byteStringToChoiceId x = Some (a, b) \<Longrightarrow> choiceIdToByteString a @ b = x"
+  apply (auto simp only:choiceIdToByteString.simps byteStringToChoiceId.simps split:option.splits prod.splits)
+  using addAndGetByteString_inverseRoundtrip append_assoc byteStringToParty_inverseRoundtrip by blast
 
 (* datatype OracleId = OracleId PubKey
 
@@ -318,6 +415,25 @@ next
 qed
 end
 (* END Proof of linorder for ValueId *)
+
+fun valueIdToByteString :: "ValueId \<Rightarrow> ByteString" where
+"valueIdToByteString (ValueId n) = packByteString n"
+
+fun byteStringToValueId :: "ByteString \<Rightarrow> (ValueId \<times> ByteString) option" where
+"byteStringToValueId x =
+  (case getByteString x of
+      None \<Rightarrow> None
+    | Some (n, t) \<Rightarrow> Some (ValueId n, t))"
+
+lemma valueIdToByteStringToValueId : "byteStringToValueId ((valueIdToByteString x) @ y) = Some (x, y)"
+  apply (cases x)
+  subgoal for n
+    using addAndGetByteString by auto
+  done
+
+lemma byteStringToValueId_inverseRoundtrip : "byteStringToValueId x = Some (a, b) \<Longrightarrow> valueIdToByteString a @ b = x"
+  apply (auto simp only:valueIdToByteString.simps byteStringToValueId.simps split:option.splits prod.splits)
+  using addAndGetByteString_inverseRoundtrip by blast
 
 datatype Value = AvailableMoney AccountId Token
                | Constant int
